WP1-Programming-Languages-Semantics/WP11-C-semantics/src/IMP-Lenses/utp_hoare_total.thy
@@ -3,7 +3,103 @@ section \<open>Verification Condition Testing\<close>
 theory utp_hoare_total
   imports "theories/utp_fault_designs"
 begin
+named_theorems hoare_total
+
+subsection {*Hoare triple definition*}
+
 definition hoare_rd :: "'\<alpha> cond \<Rightarrow> ('f,'\<alpha>) hrel_cp \<Rightarrow> '\<alpha> cond \<Rightarrow> bool" ("\<lbrace>_\<rbrace>_\<lbrace>_\<rbrace>\<^sub>D") where
 [upred_defs]:"\<lbrace>p\<rbrace>Q\<lbrace>r\<rbrace>\<^sub>D = ((\<lceil>p\<rceil>\<^sub>C\<^sub>< \<and> $ok \<and> \<not>$abrupt \<and> $fault =\<^sub>u \<guillemotleft>None\<guillemotright> \<Rightarrow> 
                           \<lceil>r\<rceil>\<^sub>C\<^sub>> \<and> $ok\<acute> \<and> \<not>$abrupt\<acute> \<and> $fault\<acute> =\<^sub>u \<guillemotleft>None\<guillemotright>) \<sqsubseteq> Q)"
+
+lemma hoare_true [hoare_total]: 
+  assumes "ok\<sharp>\<sharp>C" "abrupt\<sharp>\<sharp>C" "fault\<sharp>\<sharp>C"
+  shows "\<lbrace>p\<rbrace>C\<lbrace>true\<rbrace>\<^sub>D"
+  using assms oops
+
+lemma hoare_false [hoare_total]: "\<lbrace>false\<rbrace>C\<lbrace>q\<rbrace>\<^sub>D"
+  by rel_auto
+
+subsection {*Precondition strengthening*}
+
+lemma hoare_pre_str[hoare_total]:
+  assumes "`p\<^sub>1 \<Rightarrow> p\<^sub>2`" and "\<lbrace>p\<^sub>2\<rbrace>C\<lbrace>q\<rbrace>\<^sub>D"
+  shows "\<lbrace>p\<^sub>1\<rbrace>C\<lbrace>q\<rbrace>\<^sub>D" 
+  by (insert assms) rel_auto
+
+subsection {*Post-condition weakening*}
+
+lemma hoare_post_weak[hoare_total]:
+  assumes "\<lbrace>p\<rbrace>C\<lbrace>q\<^sub>2\<rbrace>\<^sub>D" and "`q\<^sub>2 \<Rightarrow> q\<^sub>1`"
+  shows "\<lbrace>p\<rbrace>C\<lbrace>q\<^sub>1\<rbrace>\<^sub>D" 
+ by (insert assms) rel_auto
+
+subsection {*Hoare and assertion logic*}
+
+lemma hoare_r_conj [hoare_total]: 
+  assumes"\<lbrace>p\<rbrace>C\<lbrace>r\<rbrace>\<^sub>D" and "\<lbrace>p\<rbrace>C\<lbrace>s\<rbrace>\<^sub>D"  
+  shows "\<lbrace>p\<rbrace>C\<lbrace>r \<and> s\<rbrace>\<^sub>D"
+  by (insert assms) rel_auto
+
+subsection {*Hoare SKIP*}
+
+lemma skip_hoare_r [hoare_total]: "\<lbrace>p\<rbrace>SKIP\<lbrace>p\<rbrace>\<^sub>D"
+  by rel_auto
+
+subsection {*Hoare for assignment*}
+
+lemma assigns_hoare_r [hoare_total]: 
+  assumes"`p \<Rightarrow> \<sigma> \<dagger> q`" 
+  shows  "\<lbrace>p\<rbrace>\<langle>\<sigma>\<rangle>\<^sub>C\<lbrace>q\<rbrace>\<^sub>D"
+  by (insert assms) rel_auto
+
+lemma assigns_hoare_r' [hoare_total]: "\<lbrace>\<sigma> \<dagger> p\<rbrace>\<langle>\<sigma>\<rangle>\<^sub>C\<lbrace>p\<rbrace>\<^sub>D"
+  by rel_auto
+
+subsection {*Hoare for Sequential Composition*}
+
+lemma seq_hoare_r [hoare_total]: 
+  assumes"\<lbrace>p\<rbrace>C\<^sub>1\<lbrace>s\<rbrace>\<^sub>D" and "\<lbrace>s\<rbrace>C\<^sub>2\<lbrace>r\<rbrace>\<^sub>D" 
+  shows"\<lbrace>p\<rbrace>C\<^sub>1 ;; C\<^sub>2\<lbrace>r\<rbrace>\<^sub>D"
+  by (insert assms) rel_blast
+
+subsection {*Hoare for Conditional*}
+
+lemma cond_hoare_r [hoare_total]: 
+  assumes "\<lbrace>b \<and> p\<rbrace>C\<^sub>1\<lbrace>q\<rbrace>\<^sub>D" and "\<lbrace>\<not>b \<and> p\<rbrace>C\<^sub>2\<lbrace>q\<rbrace>\<^sub>D" 
+  shows "\<lbrace>p\<rbrace>C\<^sub>1 \<triangleleft> \<lceil>b\<rceil>\<^sub>C\<^sub>< \<triangleright> C\<^sub>2\<lbrace>q\<rbrace>\<^sub>D"
+  by (insert assms) rel_blast
+
+subsection {*Hoare for assert*}
+
+lemma assert_hoare_r [hoare_total]: 
+  assumes "\<lbrace>c \<and> p\<rbrace>SKIP\<lbrace>q\<rbrace>\<^sub>D" and "\<lbrace>\<not>c \<and> p\<rbrace>\<bottom>\<^sub>D\<lbrace>q\<rbrace>\<^sub>D" 
+  shows "\<lbrace>p\<rbrace> c\<^sub>\<bottom>\<^sub>C \<lbrace>q\<rbrace>\<^sub>D"
+  by (insert assms) rel_blast
+
+subsection {*Hoare for assume*}
+
+lemma assume_hoare_r [hoare_total]: 
+  assumes "\<lbrace>c \<and> p\<rbrace>SKIP\<lbrace>q\<rbrace>\<^sub>D" and "\<lbrace>\<not>c \<and> p\<rbrace>\<top>\<^sub>D\<lbrace>q\<rbrace>\<^sub>D" 
+  shows "\<lbrace>p\<rbrace>c\<^sup>\<top>\<^sup>C\<lbrace>q\<rbrace>\<^sub>D"
+  by (insert assms) rel_blast
+
+subsection {*Hoare for While-loop*}
+
+lemma while_hoare_r [hoare_total]:
+  assumes "\<lbrace>p \<and> b\<rbrace>C\<lbrace>p\<rbrace>\<^sub>D"
+  shows "\<lbrace>p\<rbrace>WHILE b DO C OD\<lbrace>\<not>b \<and> p\<rbrace>\<^sub>D"
+  using assms
+  by (simp add: While_def hoare_rd_def, rule_tac lfp_lowerbound) (rel_blast) 
+
+lemma while_hoare_r' [hoare_total]:
+  assumes "\<lbrace>p \<and> b\<rbrace>C\<lbrace>p\<rbrace>\<^sub>D" and "`p \<and> \<not>b \<Rightarrow> q`"
+  shows "\<lbrace>p\<rbrace>WHILE b DO C OD\<lbrace>q\<rbrace>\<^sub>D"
+  using assms
+  by (metis utp_hoare_total.hoare_post_weak utp_hoare_total.while_hoare_r utp_pred.inf_commute)
+
+lemma while_invr_hoare_r [hoare_total]:
+  assumes "\<lbrace>p \<and> b\<rbrace>C\<lbrace>p\<rbrace>\<^sub>D" and "`pre \<Rightarrow> p`" and "`(\<not>b \<and> p) \<Rightarrow> post`"
+  shows "\<lbrace>pre\<rbrace>WHILE b invr p DO C OD\<lbrace>post\<rbrace>\<^sub>D"
+  by (metis assms utp_hoare_total.hoare_pre_str utp_hoare_total.while_hoare_r' utp_fault_designs.while_inv_def utp_pred.inf_commute)
+
 end
